BaseProps.v
@@ -1,0 +1,36 @@
+Require Import Morphisms Base.
+
+Definition cup x y := union (pair x y).
+
+Instance Proper_cup : Proper (V_eq ==> V_eq ==> V_eq) cup.
+Proof.
+unfold cup; repeat intro; repeat f_equiv; assumption.
+Qed.
+
+Lemma cup_spec : forall x y z, z ∈ cup x y <-> z ∈ x \/ z ∈ y.
+Proof.
+intros x y z; split; intro H.
++ apply union_spec in H; destruct H as [u [Hu Hm]].
+  apply pair_spec in Hm; destruct Hm as [Hm|Hm];
+  rewrite <- Hm; intuition.
++ apply union_spec; destruct H as [Hm|Hm].
+  - exists x; split; [assumption|apply pair_spec; left; reflexivity].
+  - exists y; split; [assumption|apply pair_spec; right; reflexivity].
+Qed.
+
+Definition cap x y := comprehension x (fun z => z ∈ y).
+
+Instance Proper_cap : Proper (V_eq ==> V_eq ==> V_eq) cap.
+Proof.
+intros x1 x2 Hx y1 y2 Hy; unfold cap; f_equiv; [assumption|].
+intros z1 z2 Hz; rewrite Hy, Hz; reflexivity.
+Qed.
+
+Lemma cap_spec : forall x y z, z ∈ cap x y <-> (z ∈ x /\ z ∈ y).
+Proof.
+intros x y z; split; intros H.
++ apply comprehension_spec in H; [|intros x1 x2 Hx; rewrite Hx; reflexivity].
+  assumption.
++ apply comprehension_spec; [|assumption].
+  intros x1 x2 Hx; rewrite Hx; reflexivity.
+Qed.
